02_FORMAL/fstar/RIINA/Properties/EffectSafety.fst
@@ -1,6 +1,6 @@
 (* Copyright (c) 2026 The RIINA Authors. All rights reserved. *)
 (* Copyright (c) 2026 The RIINA Authors. *)
-(* Derived from 02_FORMAL/coq/properties/EffectSafety.v (12 lemmas) *)
+(* Derived from 02_FORMAL/coq/properties/EffectSafety.v (32 lemmas) *)
 (* Source mapping: scripts/generate-full-stack.py *)
 module RIINA.Properties.EffectSafety
 open FStar.All
@@ -55,3 +55,63 @@ let effect_level_zero_is_pure (p_epsilon: _) : Lemma (requires (effect_level p_e
 
 (* effect_join_nonpure (matches Coq: Lemma effect_join_nonpure) *)
 let effect_join_nonpure (p_epsilon1: _) (p_epsilon2: _) : Lemma (requires (~(p_epsilon2 == EffPure))) (ensures (~(effect_join p_epsilon1 p_epsilon2 == EffPure))) = admit ()
+
+(* effect_join_monotone (matches Coq: Lemma effect_join_monotone) *)
+let effect_join_monotone (p_epsilon1: _) (p_epsilon1_: _) (p_epsilon2: _) (p_epsilon2_: _) : Lemma (requires (effect_leq p_epsilon1 p_epsilon1_ == true /\ effect_leq p_epsilon2 p_epsilon2_ == true)) (ensures (effect_leq (effect_join p_epsilon1 p_epsilon2) (effect_join p_epsilon1_ p_epsilon2_) == true)) = admit ()
+
+(* effect_join_mono_l (matches Coq: Lemma effect_join_mono_l) *)
+let effect_join_mono_l (p_epsilon1: _) (p_epsilon1_: _) (p_epsilon2: _) : Lemma (requires (effect_leq p_epsilon1 p_epsilon1_ == true)) (ensures (effect_leq (effect_join p_epsilon1 p_epsilon2) (effect_join p_epsilon1_ p_epsilon2) == true)) = admit ()
+
+(* effect_join_mono_r (matches Coq: Lemma effect_join_mono_r) *)
+let effect_join_mono_r (p_epsilon1: _) (p_epsilon2: _) (p_epsilon2_: _) : Lemma (requires (effect_leq p_epsilon2 p_epsilon2_ == true)) (ensures (effect_leq (effect_join p_epsilon1 p_epsilon2) (effect_join p_epsilon1 p_epsilon2_) == true)) = admit ()
+
+(* effect_leq_pure (matches Coq: Lemma effect_leq_pure) *)
+let effect_leq_pure (p_epsilon: _) : Lemma (effect_leq EffPure p_epsilon == true) = admit ()
+
+(* read_leq_write (matches Coq: Lemma read_leq_write) *)
+let read_leq_write () : Lemma (effect_leq EffRead EffWrite == true) = admit ()
+
+(* write_subsumes_read (matches Coq: Lemma write_subsumes_read) *)
+let write_subsumes_read () : Lemma (effect_join EffRead EffWrite == EffWrite) = admit ()
+
+(* write_leq_filesystem (matches Coq: Lemma write_leq_filesystem) *)
+let write_leq_filesystem () : Lemma (effect_leq EffWrite EffFileSystem == true) = admit ()
+
+(* pure_leq_read (matches Coq: Lemma pure_leq_read) *)
+let pure_leq_read () : Lemma (effect_leq EffPure EffRead == true) = admit ()
+
+(* pure_leq_write (matches Coq: Lemma pure_leq_write) *)
+let pure_leq_write () : Lemma (effect_leq EffPure EffWrite == true) = admit ()
+
+(* read_neq_write (matches Coq: Lemma read_neq_write) *)
+let read_neq_write () : Lemma (~(EffRead == EffWrite)) = admit ()
+
+(* effect_join_pure_l (matches Coq: Lemma effect_join_pure_l) *)
+let effect_join_pure_l (p_epsilon: _) : Lemma (effect_join EffPure p_epsilon == p_epsilon) = admit ()
+
+(* effect_join_idem (matches Coq: Lemma effect_join_idem) *)
+let effect_join_idem (p_epsilon: _) : Lemma (effect_join p_epsilon p_epsilon == p_epsilon) = admit ()
+
+(* base_value_always_pure (matches Coq: Lemma base_value_always_pure) *)
+let base_value_always_pure (p_gamma: _) (p_sigma: _) (p_delta: _) (p_v: _) (p_t: _) (p_epsilon: _) : Lemma (requires (has_type p_gamma p_sigma p_delta p_v p_t p_epsilon == true /\ (p_v == EUnit \/ ((exists p_b. p_v == EBool p_b)) \/ ((exists p_n. p_v == EInt p_n)) \/ ((exists p_s. p_v == EString p_s)) \/ ((exists p_l. p_v == ELoc p_l)) \/ ((exists p_x. (exists p_t. p_v == ELam p_x p_t' body)))))) (ensures (p_epsilon == EffPure)) = admit ()
+
+(* pure_multi_step_preserves_ctx (matches Coq: Theorem pure_multi_step_preserves_ctx) *)
+let pure_multi_step_preserves_ctx (p_e: _) (p_e_: _) (p_t: _) (p_st: _) (p_st_: _) (p_ctx: _) (p_ctx_: _) (p_sigma: _) : Lemma (requires (has_type [] p_sigma Public p_e p_t EffPure == true /\ store_wf p_sigma p_st == true /\ step (p_e, p_st, p_ctx) * (p_e_, p_st_, p_ctx_) == true)) (ensures (p_ctx_ == p_ctx)) = admit ()
+
+(* effect_read_not_pure (matches Coq: Lemma effect_read_not_pure) *)
+let effect_read_not_pure () : Lemma (~(EffRead == EffPure)) = admit ()
+
+(* effect_write_not_pure (matches Coq: Lemma effect_write_not_pure) *)
+let effect_write_not_pure () : Lemma (~(EffWrite == EffPure)) = admit ()
+
+(* effect_filesystem_not_pure (matches Coq: Lemma effect_filesystem_not_pure) *)
+let effect_filesystem_not_pure () : Lemma (~(EffFileSystem == EffPure)) = admit ()
+
+(* effect_network_not_pure (matches Coq: Lemma effect_network_not_pure) *)
+let effect_network_not_pure () : Lemma (~(EffNetwork == EffPure)) = admit ()
+
+(* effect_system_not_pure (matches Coq: Lemma effect_system_not_pure) *)
+let effect_system_not_pure () : Lemma (~(EffSystem == EffPure)) = admit ()
+
+(* effect_crypto_not_pure (matches Coq: Lemma effect_crypto_not_pure) *)
+let effect_crypto_not_pure () : Lemma (~(EffCrypto == EffPure)) = admit ()
